through start of take

lists.dfy
@@ -1,3 +1,5 @@
+// Nil: empty list
+// Cons: non-empty list (Node)
 datatype List<A> = Nil | Cons(head: A, tail: List<A>)
 
 // []: Nil
@@ -9,6 +11,64 @@ datatype List<A> = Nil | Cons(head: A, tail: List<A>)
 // Cons(_, tail): length(tail) + 1
 function method length<A>(list: List<A>): int
 	ensures length(list) >= 0;
+	ensures has_length(list, length(list));
 {
 	if (list.Nil?) then 0 else length(list.tail) + 1
+}
+
+predicate has_length<A>(list: List<A>, len: int)
+{
+	(list.Nil? ==> len == 0) &&
+  (list.Cons? ==> exists restLen :: has_length(list.tail, restLen) && len == restLen + 1)
+}
+
+ghost method length_works_correctly()
+{
+	var nil: List<int> := Nil;
+	assert length(nil) == 0;
+	assert length(Cons(0, Nil)) == 1;
+	assert length(Cons(0, Cons(1, Nil))) ==  2;
+	assert length(Cons(0, Cons(1, Cons(2, Nil)))) == 3;
+}
+
+// issues:
+//   -index could get negative
+//   -index could be too big
+//
+// getElementAtIndex(Nil, 0)
+// getElementAtIndex(Cons(1, Cons(2, Nil)), 5)
+//
+function method getElementAtIndex<A>(list: List<A>, index: int): A
+	requires 0 <= index < length(list);
+	ensures is_element_at_index(list, index, getElementAtIndex(list, index));
+{
+	if (index == 0) then list.head else getElementAtIndex(list.tail, index - 1)
+}
+
+predicate is_element_at_index<A>(list: List<A>, index: int, element: A)
+	requires 0 <= index < length(list);
+{
+	(index == 0 ==> list.head == element) &&
+  (index > 0 ==> is_element_at_index(list.tail, index - 1, element))
+}
+
+ghost method testGetElementAtIndex() {
+	assert getElementAtIndex(Cons(1, Nil), 0) == 1;
+	assert getElementAtIndex(Cons(2, Cons(1, Nil)), 1) == 1;
+	assert getElementAtIndex(Cons(2, Cons(1, Nil)), 0) == 2;
+}
+
+// Cons(1, Cons(2, Cons(3, Nil))): [1, 2, 3]
+// take([1, 2, 3], 0) == []
+// take([1, 2, 3], 1) == [1]
+// take([1, 2, 3], 2) == [1, 2]
+// take([5, 6, 3], 2) == [5, 6]
+// take([5, 6, 2], 3) == [5, 6, 2]
+//
+// take([2, 1, 3], -1) == <<INVALID>>
+// take([9, 3, 4], 5) == <<INVALID>>
+//
+function method take<A>(list: List<A>, amount: int): List<A>
+	requires 0 <= amount <= length(list);
+{
 }
